almost done with transitivity prover

src/ndep/Provers.v
@@ -3,6 +3,8 @@ Require Import Bedrock.ndep.Expr.
 Require Import EquivDec.
 Require Import Env.
 
+Set Implicit Arguments.
+
 Notation "[ a ]" := (a :: nil).
 Notation "[ a ,  b ]" := (a :: b :: nil).
 Notation "[ a ,  b ,  c ]" := (a :: b :: c :: nil).
@@ -22,14 +24,26 @@ Section ProverT.
    * but that is harder to program with
    *)
 
+  Definition ValidProp (e : expr types) := ~ exprD fs nil nil e tvProp = None.
+
+  Lemma Provable_ValidProp : forall goal, Provable fs nil nil goal -> ValidProp goal.
+    intros.
+    unfold Provable, ValidProp in *.
+    destruct (exprD fs nil nil goal tvProp); intuition.
+    discriminate.
+  Qed.
+  
+  Definition ProverCorrect (prover : list (@expr types) -> @expr types -> bool) :=
+    forall hyps goal, prover hyps goal = true ->
+      ValidProp goal ->
+      AllProvable fs nil nil hyps ->
+      Provable fs nil nil goal.
+
   (* the non-dependent prover should be *)
   Record NProverT : Type :=
-  { prove : forall  (hyps : list (@expr types)) (goal : @expr types), bool
-  ; prove_correct : 
-    forall hyps goal, 
-    prove hyps goal = true ->
-    AllProvable fs nil nil hyps ->
-    Provable fs nil nil goal
+  {
+    prove : forall (hyps : list (@expr types)) (goal : @expr types), bool;
+    prove_correct : ProverCorrect prove
   }.
 
 End ProverT.
@@ -39,7 +53,6 @@ Definition eq_dec_to_seq_dec A (d : forall x y : A, { x = y } + { ~ x = y }) x y
        | left pf => Some pf
        | right _ => None
      end.
-Implicit Arguments eq_dec_to_seq_dec [A].
 
 Require Import Arith Bool.
 Definition type_nat := {| Expr.Eq := eq_dec_to_seq_dec eq_nat_dec |}.
@@ -51,100 +64,761 @@ Definition tvar_nat := tvType 0.
 Definition tvar_bool := tvType 1.
 Definition tvar_list_bool := tvType 2.
 Definition tvar_empty := tvType 3.
-Check Build_signature.
-Definition test_eq_sig := Build_signature test_types [tvar_nat, tvar_nat] tvar_bool beq_nat.
-Definition test_plus_sig := Build_signature test_types [tvar_nat, tvar_nat] tvar_nat plus.
+Definition test_eq_sig := Sig test_types [tvar_nat, tvar_nat] tvar_bool beq_nat.
+Definition test_plus_sig := Sig test_types [tvar_nat, tvar_nat] tvar_nat plus.
 Fixpoint bin_to_nat (ls : list bool) : nat :=
   match ls with
     | nil => 0
     | false :: ls' => 2 * (bin_to_nat ls')
     | true :: ls' => S (2 * (bin_to_nat ls'))
   end.
-Definition test_bin_to_nat_sig := Build_signature test_types [tvar_list_bool] tvar_nat bin_to_nat.
-Definition test_constant_false_sig := Build_signature test_types [tvar_empty] tvar_bool (fun _ => false).
+Definition test_bin_to_nat_sig := Sig test_types [tvar_list_bool] tvar_nat bin_to_nat.
+Definition test_constant_false_sig := Sig test_types [tvar_empty] tvar_bool (fun _ => false).
 Definition test_functions := [test_eq_sig, test_plus_sig, test_bin_to_nat_sig, test_constant_false_sig].
 (* 0 => eq, 1 => plus, 2 => bin_to_nat, 3 => fun _ => false *)
 Eval compute in (Denotation test_eq_sig).
 Eval compute in (functionTypeD (map (tvarD test_types) (Domain test_eq_sig))
          (tvarD test_types (Range test_eq_sig))).
 
+Hint Unfold ProverCorrect ValidProp Provable : provers.
+Ltac prover2 := intros; autounfold with provers in *; intros;
+  match goal with
+    | [ hyps : list (@expr _) |- _ ] => induction hyps
+  end; simpl in *; try discriminate;
+  match goal with
+    | _ => pose 4
+  end.
+
 Section AssumptionProver.
   Variable types : list type.
   Variable fs : functions types.
 
-  Fixpoint assumptionProver hyps (goal : expr types) 
-    : AllProvable fs nil nil hyps 
-    -> option (Provable fs nil nil goal) :=
+  Fixpoint assumptionProver (hyps : list (expr types)) (goal : expr types) : bool :=
     match hyps with
-      | nil => fun _ => None
-      | exp :: b => fun pfHyps : AllProvable fs nil nil (exp :: b) =>
-        match seq_dec exp goal with
-          | Some pf => Some match pf in _ = t return Provable fs nil nil t with
-                              | refl_equal => proj1 pfHyps
-                            end
-          | None => assumptionProver b goal (proj2 pfHyps)
-        end
+      | nil => false
+      | exp :: b => if seq_dec exp goal then true else false
     end.
+
+  Theorem assumptionProverCorrect : ProverCorrect fs assumptionProver.
+    prover2.
+    destruct (expr_seq_dec a goal).
+    subst.
+    intuition.
+    discriminate.
+  Qed.
+
+  Definition assumptionProverRec := {| prove := assumptionProver; prove_correct := assumptionProverCorrect |}.
 End AssumptionProver.
+
+Section UpdatePosition.
+  Variable A : Type.
+  
+  Fixpoint updatePosition (ls : list A) (n : nat) (new : A) : list A :=
+    match ls with
+      | nil => match n with
+                 | 0 => [new]
+                 | S n' => new :: updatePosition nil n' new
+               end
+      | a :: ls' => match n with
+                      | 0 => new :: ls'
+                      | S n' => a :: updatePosition ls' n' new
+                    end
+    end.
+
+  Require Import Omega.
+  Hint Resolve lt_n_O.
+  Lemma nth_error_updatePosition_nil : forall (new : A) n, nth_error (updatePosition nil n new) n = value new.
+    intros.
+    induction n; auto.
+  Qed.
+  Hint Resolve nth_error_updatePosition_nil.
+  Lemma nth_error_updatePosition : forall (new : A) ls n, nth_error (updatePosition ls n new) n = value new.
+    intro.
+    double induction ls n; auto.
+    intros.
+    specialize (H0 H).
+    simpl.
+    destruct l0; auto.
+  Qed.
+End UpdatePosition.
+
+Ltac caseDestruct t := destruct t; try discriminate.
+
+Ltac dintuition := repeat (intuition;
+  match goal with
+    | [ H : exists _, _ |- _ ] => destruct H
+  end).
+
+Ltac hypRewriter := repeat match goal with
+                             | [ H : _ = _ |- _] => rewrite H
+                           end.
+Ltac unlet := repeat match goal with
+                       | [ x := ?y |- _ ] => subst x
+                     end.
+
+Ltac provers := unlet; repeat (repeat (autorewrite with provers in *; hypRewriter); simpl in *; subst; dintuition); try congruence; firstorder.
 
 Section ReflexivityProver.
   Context {types : list type}.
   Variable fs : functions types.
-  Variable eqFun : func.
-  
-  Definition reflexivityProver : (@ProverT types) := fun hyps goal => 
+  Variable eqFunIdx : func.
+  Variable eqFunTvar : tvar.
+
+  Let eqFunSig := {| Domain := [eqFunTvar, eqFunTvar]; Range := tvProp; Denotation := (@eq (tvarD types eqFunTvar)) |}.
+  Let fs' := updatePosition fs eqFunIdx eqFunSig.
+
+  Definition reflexivityProver (hyps : list (expr types)) (goal : expr types) := 
     match goal with
-      | Func f [x, y] => if equiv_dec f eqFun
+      | Func f [x, y] => if equiv_dec f eqFunIdx
                            then if expr_seq_dec x y then true else false
                            else false
       | _ => false
     end.
 
-  Check (nth_error test_functions 0).
-
-  Ltac caseDestruct t := destruct t; try discriminate.
-  Theorem reflexivityProverOk : ProverCorrect fs reflexivityProver.
-    unfold ProverCorrect.
-    intros.
-    unfold FalseDefault.
-    unfold reflexivityProver in H.
+  Hint Rewrite nth_error_updatePosition : provers.
+  Theorem reflexivityProverCorrect : ProverCorrect fs' reflexivityProver.
+    unfold ProverCorrect; intros.
     caseDestruct goal.
     repeat caseDestruct l.
-    caseDestruct (equiv_dec f eqFun).
+    simpl in *.
+    caseDestruct (equiv_dec f eqFunIdx).
     unfold equiv in *.
     caseDestruct (expr_seq_dec e e0).
+    subst.
+    unfold fs', exprD, Provable.
+    simpl.
+    rewrite nth_error_updatePosition.
+    simpl.
+    unfold ValidProp in *.
+    unfold fs' in *.
+    case_eq (exprD (updatePosition fs eqFunIdx eqFunSig) nil nil e0 eqFunTvar); intros.
+    reflexivity.
+    apply H0.
+    provers.
   Qed.
-  
+
+  Definition reflexivityProverRec := {| prove := reflexivityProver; prove_correct := reflexivityProverCorrect |}.
 End ReflexivityProver.
 
+(* Algorithm for grouping expressions by equalities. Terribly inefficient... *)
+Section Grouper.
+  Variable A : Type.
+  Variable A_seq_dec : forall (x y : A), option (x = y).
+  
+  Definition in_seq_dec (ls : list A) (a : A) : option (In a ls).
+    induction ls.
+    right.
+    simpl.
+    destruct IHls.
+    left.
+    tauto.
+    destruct (A_seq_dec a0 a).
+    left.
+    tauto.
+    right.
+  Defined.
+
+  Fixpoint groupWith (grps : list (list A)) (g : list A) (a : A) :=
+    match grps with
+      | nil => [g]
+      | g' :: grps' => if in_seq_dec g' a
+                         then groupWith grps' (g' ++ g) a
+                         else g' :: groupWith grps' g a
+    end.
+
+  Fixpoint addEquality (ls : list (list A)) (a : A) (b : A) : list (list A) :=
+    match ls with
+      | nil => [[a]] (* matched nothing *)
+      | grp :: ls' => if in_seq_dec grp a
+                        then groupWith ls' grp b
+                        else if in_seq_dec grp b
+                               then groupWith ls' grp a
+                               else grp :: addEquality ls' a b
+    end.
+
+  Fixpoint inSameGroup (grps : list (list A)) (a : A) (b : A) :=
+    if A_seq_dec a b
+      then true
+      else
+        match grps with
+          | nil => false
+          | g :: grps' => if in_seq_dec g a
+                            then
+                              if in_seq_dec g b
+                                then true
+                                else inSameGroup grps' a b
+                            else inSameGroup grps' a b
+        end.    
+
+  Fixpoint groupEqualTo (g : list A) a :=
+    match g with
+      | nil => True
+      | a' :: g' => a = a' /\ groupEqualTo g' a
+    end.
+
+  Lemma groupEqualTo_spec : forall (g : list A) a, groupEqualTo g a <-> (forall x, In x g -> a = x).
+    intros; split; induction g; simpl in *; intuition; try congruence.
+  Qed.
+    
+  Definition groupEqual (g : list A) :=
+    match g with
+      | nil => True
+      | a' :: g' => groupEqualTo g' a'
+    end.
+
+  Lemma groupEqualTo_groupEqual : forall (g : list A) a, groupEqualTo g a -> groupEqual g.
+    induction g; simpl in *; intuition; subst; intuition.
+  Qed.
+
+  Hint Resolve groupEqualTo_groupEqual.
+  Lemma groupEqual_spec : forall (g : list A), groupEqual g <-> forall x y, In x g -> In y g -> x = y.
+    intros; split; intros.
+    induction g.
+    intuition.
+    simpl in *.
+    destruct (groupEqualTo_spec g a).
+    intuition.
+    congruence.
+    specialize (H1 _ H0); congruence.
+    specialize (H1 _ H4); congruence.
+    pose groupEqualTo_groupEqual.
+    firstorder.
+    induction g.
+    provers.
+    simpl in *; intuition.
+    apply groupEqualTo_spec.
+    intuition.
+  Qed.
+
+  Lemma groupEqual_app : forall g1 g2, groupEqual g1 -> groupEqual g2 -> (exists a, In a g1 /\ In a g2) -> groupEqual (g1 ++ g2).
+    intros ? ? Hg1 Hg2 Hex.
+    apply groupEqual_spec.
+    destruct Hex.
+    intuition.
+    destruct (groupEqual_spec g1), (groupEqual_spec g2).
+    repeat match goal with
+      | [ H : In _ (_ ++ _) |- _ ] => destruct (in_app_or _ _ _ H); clear H
+    end; intuition;
+    repeat match goal with
+      | [ H1 : In ?x ?g, H2 : In ?y ?g, H3 : groupEqual ?g |- _ ] =>
+          match goal with
+            | [ H : x = y |- _ ] => fail 1
+            | [ H : y = x |- _ ] => fail 1
+            | _ => assert (x = y) by intuition
+          end
+    end; congruence.
+  Qed.
+
+  Fixpoint groupsEqual (grps : list (list A)) :=
+    match grps with
+      | nil => True
+      | g :: grps' => groupEqual g /\ groupsEqual grps'
+    end.
+
+  Ltac solve_spec := repeat (simpl in *; subst; intuition); try congruence; firstorder.
+  
+  Lemma groupsEqual_spec : forall (grps : list (list A)), groupsEqual grps <-> forall g, In g grps -> forall x y, In x g -> In y g -> x = y.
+    induction grps; pose groupEqual_spec; solve_spec.
+  Qed.
+
+  Lemma groupsEqual_groupWith : forall grps, groupsEqual grps -> forall g, groupEqual g -> forall a, In a g -> groupsEqual (groupWith grps g a).
+    induction grps; simpl in *; intuition.
+    destruct (in_seq_dec a a0).
+    apply H.
+    apply groupEqual_app; firstorder.
+    Hint Resolve in_or_app.
+    eauto.
+    simpl in *; intuition.
+  Qed.
+
+  Lemma groupsEqual_addEquality : forall grps, groupsEqual grps -> forall x y, x = y -> groupsEqual (addEquality grps x y).
+    induction grps; solve_spec.
+    case_eq (in_seq_dec a y); intros.
+    apply groupsEqual_groupWith; solve_spec.
+    solve_spec.
+  Qed.
+
+  Lemma inSameGroup_spec : forall x y grps, inSameGroup grps x y = true <-> (exists pf, A_seq_dec x y = Some pf) \/ exists g, In g grps /\ (exists pfx, in_seq_dec g x = Some pfx) /\ (exists pfy, in_seq_dec g y = Some pfy).
+    solve_spec.
+    case_eq (A_seq_dec x y); intros.
+    left.
+    exists e; reflexivity.
+    right.
+    induction grps.
+    simpl in *.
+    rewrite H0 in H.
+    intuition.
+    simpl in *.
+    rewrite H0 in H.
+    case_eq (in_seq_dec a x); intros; rewrite H1 in H.
+    case_eq (in_seq_dec a y); intros; rewrite H2 in H.
+    firstorder.
+    firstorder.
+    firstorder.
+    destruct grps; simpl in *; rewrite H; intuition.
+    induction grps; simpl in *; intuition;
+    case_eq (A_seq_dec x y); intuition; subst.
+    rewrite H0, H1; intuition.
+    destruct (in_seq_dec a x); destruct (in_seq_dec a y); intuition.
+  Qed.
+
+  Lemma inSameGroup_addEquality : forall x y grps, A_seq_dec x y <> None -> inSameGroup (addEquality grps x y) x y = true.
+    intros.
+    case_eq (A_seq_dec x y); intuition.
+    subst.
+    induction grps.
+    simpl; intuition.
+    repeat rewrite H0; intuition.
+    destruct (addEquality (a :: grps) y y); simpl; rewrite H0; intuition.
+  Qed.
+
+  Lemma in_seq_dec_spec : forall x g, (exists pf, in_seq_dec g x = Some pf) <-> In x g /\ exists pf, A_seq_dec x x = Some pf.
+    dintuition.
+    induction g; intuition.
+    simpl in *; intuition.
+    destruct x0; intuition.
+    subst.
+    destruct (in_seq_dec g x); intuition.
+    apply (IHg i); intuition.
+    destruct (A_seq_dec x x); intuition.
+    exists e; intuition.
+    discriminate.
+    destruct (in_seq_dec g x).
+    apply (IHg i0); intuition.
+    case_eq (A_seq_dec a x); intros.
+    subst.
+    rewrite H0.
+    exists eq_refl.
+    reflexivity.
+    rewrite H0 in H.
+    discriminate.
+    induction g.
+    intuition.
+    simpl in *; intuition.
+    destruct (in_seq_dec g x).
+    exists (or_intror (a = x) i); reflexivity.
+    subst.
+    exists (or_introl (In x g) x0).
+    rewrite H; reflexivity.
+    dintuition.
+    rewrite H0.
+    exists (or_intror (a = x) x1).
+    reflexivity.
+  Qed.
+    
+  Lemma in_seq_dec_app : forall x g g', (exists pfl, in_seq_dec g x = Some pfl) -> exists pfr, in_seq_dec (g' ++ g) x = Some pfr.
+    dintuition.
+    induction g'.
+    simpl in *; firstorder.
+    simpl in *.
+    destruct IHg'.
+    rewrite H0.
+    exists (or_intror (a = x) x1); intuition.
+  Qed.
+
+  Lemma in_seq_dec_app_r : forall x g g', (exists pfl, in_seq_dec g x = Some pfl) -> exists pfr, in_seq_dec (g ++ g') x = Some pfr.
+    intros.
+    apply in_seq_dec_app with (g' := g') in H.
+    pose in_seq_dec_spec.
+    destruct (i x (g' ++ g)).
+    apply in_seq_dec_spec.
+    intuition.
+    apply in_or_app.
+    apply in_app_or in H0.
+    intuition.
+  Qed.
+
+  Lemma in_impl_in_seq_dec_impl : forall g g', (forall y, In y g -> In y g') -> forall y, (exists pf, in_seq_dec g y = Some pf) -> exists pf', in_seq_dec g' y = Some pf'.
+    intros.
+    apply in_seq_dec_spec.
+    destruct (in_seq_dec_spec y g).
+    solve_spec.
+  Qed.
+
+  Lemma groupWith_spec1 : forall grps g, In g grps -> forall x, in_seq_dec g x = None -> forall g', In g (groupWith grps g' x).
+    induction grps; solve_spec.
+    rewrite H; solve_spec.
+    destruct (in_seq_dec a x); solve_spec.
+  Qed.
+
+  Lemma groupWith_last : forall grps g x y, In y g -> In y (last (groupWith grps g x) nil).
+    induction grps; solve_spec.
+    destruct (in_seq_dec a x).
+    intuition.
+    simpl.
+    specialize (IHgrps g x y).
+    destruct (groupWith grps g x); simpl in *; intuition.
+  Qed.
+
+  Lemma groupWith_last_in_seq_dec : forall grps g x y, (exists pf, in_seq_dec g y = Some pf) -> exists pf, in_seq_dec (last (groupWith grps g x) nil) y = Some pf.
+    induction grps; solve_spec.
+    destruct (IHgrps g x y (ex_intro _ _ H)).
+    apply in_seq_dec_spec; intuition.
+    destruct (in_seq_dec a x).
+    apply groupWith_last.
+    solve_spec.
+    solve_spec.
+    destruct (groupWith grps g x); solve_spec.
+    destruct (in_seq_dec_spec y g).
+    solve_spec.
+  Qed.
+
+  Lemma groupWith_nil : forall grps g x, groupWith grps g x <> nil.
+    induction grps; solve_spec.
+    destruct (in_seq_dec a x); solve_spec.
+  Qed.
+
+  Lemma last_in : forall B (l : list B) b, l <> nil -> In (last l b) l.
+    induction l; solve_spec.
+    destruct l.
+    solve_spec.
+    right.
+    apply IHl.
+    solve_spec.
+  Qed.
+
+  Lemma groupWith_spec2 : forall grps g, In g grps -> forall x, (exists pf, in_seq_dec g x = Some pf) -> forall g1, exists g', In g' (groupWith grps g1 x) /\  forall y, In y g -> In y g'.
+    intros.
+    exists (last (groupWith grps g1 x) nil).
+    solve_spec.
+    case_eq (groupWith grps g1 x); intros.
+    apply groupWith_nil in H1; intuition.
+    apply last_in; solve_spec.
+    revert grps g H x g1 y H1 x0 H0.
+    induction grps.
+    solve_spec.
+    intros.
+    simpl in *; intuition.
+    subst.
+    rewrite H0.
+    apply groupWith_last; solve_spec.
+    destruct (in_seq_dec a x).
+    eapply IHgrps; eauto.
+    simpl.
+    case_eq (groupWith grps g1 x); intros.
+    apply groupWith_nil in H; intuition.
+    rewrite <- H.
+    eapply IHgrps; eauto.
+  Qed.
+
+  Lemma groupWith_groups : forall grps g, In g grps -> forall g1 x, exists g2, In g2 (groupWith grps g1 x) /\ (forall y, In y g -> In y g2).
+    intros.
+    case_eq (in_seq_dec g x); intros.
+    apply groupWith_spec2; solve_spec.
+    exists g; split.
+    apply groupWith_spec1; solve_spec.
+    solve_spec.
+  Qed.
+
+  Hint Resolve last_in groupWith_nil groupWith_last.
+  Lemma groupWith_arg : forall grps g x, exists g', In g' (groupWith grps g x) /\ forall y, In y g -> In y g'.
+    intros.
+    exists (last (groupWith grps g x) nil); intuition eauto.
+  Qed.
+
+  Hint Rewrite plus_assoc : null.
+  Lemma inSameGroup_refl : forall grps x, (exists pf, A_seq_dec x x = Some pf) -> inSameGroup grps x x = true.
+    induction grps; solve_spec; rewrite H; reflexivity.
+  Qed.
+    
+  Hint Resolve groupWith_last_in_seq_dec in_seq_dec_app_r.
+  Lemma inSameGroup_groupWith : forall grps x y, inSameGroup grps x y = true -> forall g z, inSameGroup (groupWith grps g z) x y = true.
+    intros.
+    apply inSameGroup_spec.
+    case_eq (A_seq_dec x y); intros; [ left | right ].
+    exists e; solve_spec.
+    revert grps x y H g z H0.
+    induction grps; intuition;
+    simpl in *;
+    rewrite H0 in H; intuition.
+    case_eq (in_seq_dec a z); intros.
+    case_eq (in_seq_dec a x); intros;
+    rewrite H2 in *.
+    case_eq (in_seq_dec a y); intros;
+    rewrite H3 in *.
+    exists (last (groupWith grps (a ++ g) z) nil); intuition;
+    apply (groupWith_last_in_seq_dec);
+    apply in_seq_dec_app_r; firstorder.
+    intuition eauto.
+    intuition eauto.
+    case_eq (in_seq_dec a x); intros.
+    case_eq (in_seq_dec a y); intros.
+    exists a.
+    solve_spec.
+    rewrite H2, H3 in *.
+    destruct (IHgrps x y H g z); try assumption.
+    solve_spec.
+    rewrite H2 in *.
+    destruct (IHgrps x y H g z); try assumption.
+    solve_spec.
+  Qed.
+
+  Hint Resolve inSameGroup_groupWith in_impl_in_seq_dec_impl.
+  Theorem inSameGroup_addEquality_preserved : forall x y grps, inSameGroup grps x y = true -> forall w z, inSameGroup (addEquality grps w z) x y = true.
+    induction grps; solve_spec.
+    destruct (A_seq_dec x y); solve_spec.
+    case_eq (A_seq_dec x y); intros.
+    match goal with
+      | [ |- inSameGroup ?l _ _ = true ] => destruct l
+    end; solve_spec; rewrite H0 in *; intuition.
+    rewrite H0 in *.
+    case_eq (in_seq_dec a x); intros;
+    rewrite H1 in *.
+    case_eq (in_seq_dec a y); intros;
+    rewrite H2 in *.
+    case_eq (in_seq_dec a w); intros.
+    apply inSameGroup_spec.
+    right.
+    destruct (groupWith_arg grps a z).
+    exists x0.
+    intuition eauto.
+    destruct (in_seq_dec a z).
+    apply inSameGroup_spec.
+    right.
+    destruct (groupWith_arg grps a w).
+    exists x0.
+    intuition eauto.
+    simpl.
+    rewrite H0, H1, H2; reflexivity.
+    destruct (in_seq_dec a w).
+    eauto.
+    destruct (in_seq_dec a z).
+    eauto.
+    simpl.
+    rewrite H0, H1, H2.
+    eauto.
+    destruct (in_seq_dec a w).
+    eauto.
+    destruct (in_seq_dec a z).
+    eauto.
+    simpl.
+    rewrite H0, H1.
+    eauto.
+  Qed.
+End Grouper.
+
 Section BabyOmega.
-  Context {types : list type}.
-  Context {fs : forall types', functions (types' ++ types)}.
+  Hint Rewrite nth_error_updatePosition : provers.
+  
+  Variable types : list type.
+  Variable natIdx : nat.
+  Let natType := {| Expr.Eq := eq_dec_to_seq_dec eq_nat_dec |}.
+  Let types' := updatePosition types natIdx natType.
+  Variable fs : functions types'.
+  Variable eqFunIdx : nat.
+  Let natTvar := tvType natIdx.
+  
+  Let eqFunSig := {| Domain := [natTvar, natTvar]; Range := tvProp; Denotation := (@eq (tvarD types' natTvar)) |}.
+  Let fs' := updatePosition fs eqFunIdx eqFunSig.
 
-  Definition types' : list type :=
-    {| Impl := nat; Expr.Eq := fun x y : nat => match Peano_dec.eq_nat_dec x y with left Heq => Some Heq | _ => None end |} :: types.
+  (*Fixpoint cast' (P : option type -> Type) natIdx types : P (nth_error types' natIdx) -> P (Some natType) :=
+  match natIdx with
+    | O => fun x => x
+    | S natIdx' => match types
+                     return P (nth_error (updatePosition types (S natIdx') natType)
+                       (S natIdx')) -> _ with
+                     | nil => cast' P natIdx' nil
+                     | _ => cast' P natIdx' _
+                   end
+  end.*)
+  
 
-  Definition fs' : functions types' :=
-    (@Sig types' (tvType 0 :: tvType 0 :: nil) tvProp (@eq nat)) ::
-    (@Sig types' (tvType 0 :: tvType 0 :: nil) (tvType 0) plus) ::
-    fs (_ :: nil).
+  Definition nat_seq_dec := eq_dec_to_seq_dec eq_nat_dec.
+  
+  Definition optionDefault T (o : option T) t :=
+    match o with
+      | Some pf => pf
+      | None => t
+    end.
 
-  Definition BabyOmega : @ProverT types' fs'.
-    red.
-    refine (fun _ goal _ => None).
-(*
-      match goal in expr _ _ _ T return option (match T return expr _ _ _ T -> Type with
-                                                | tvProp => fun goal => exprD HNil HNil goal
-                                                | _ => fun _ => Empty_set
-                                              end goal) with
-        | Func f args =>
-          finIfz f DMatch
-            (fun args => hlistDestruct args (DMatch' _) 
-              (fun x y => if seq_dec x y then Some _ else None))
-            (fun _ _ => None) args
-        | _ => None
-      end);
-    try abstract congruence.
-*)
-    Defined.
+  Definition natTvarCoerce (n : nat) : tvarD types' natTvar.
+    simpl.
+    subst types'.
+    rewrite nth_error_updatePosition.
+    simpl.
+    exact n.
+  Defined.
+
+  Lemma nth_error_types'_natIdx : nth_error types' natIdx = value {| Expr.Eq := eq_dec_to_seq_dec eq_nat_dec |}.
+    provers.
+  Qed.
+  Hint Rewrite nth_error_types'_natIdx : provers.
+  
+  Definition natTvarCoerceR (n : tvarD types' natTvar) : nat.
+    simpl in *.
+    rewrite nth_error_types'_natIdx in *.
+    simpl in *.
+    exact n.
+  Defined.
+
+  (*Lemma natTvarCoerceR_natTvarCoerce : forall n, natTvarCoerceR (natTvarCoerce n) = n.
+    induction n.
+    unfold natTvarCoerce.
+    unfold eq_rect_r, eq_rect.
+    generalize (nth_error (updatePosition types natIdx
+           {| Impl := nat; Expr.Eq := eq_dec_to_seq_dec eq_nat_dec |}) natIdx).
+    generalize (Logic.eq_sym
+         (nth_error_updatePosition
+            {| Impl := nat; Expr.Eq := eq_dec_to_seq_dec eq_nat_dec |} types
+            natIdx)).
+    intro.
+
+    case e.
+    generalize {| Impl := nat; Expr.Eq := eq_dec_to_seq_dec eq_nat_dec |}.
+    intro.
+    destruct e.
+    rewrite nth_error_updatePosition.
+    pose (NatEqdep.UIP_refl 0).*)
+
+  Lemma natTvarCoerceR_inj : forall m n, natTvarCoerceR m = natTvarCoerceR n -> m = n.
+  Admitted.
+    (*simpl in *.
+    unfold natTvarCoerceR in H.
+    assert (match nth_error types' natIdx with
+      | Some t => Impl t
+      | None => Empty_set
+      end = nat) by provers.
+    simpl in H.
+    rewrite H0 in H.
+    elim (nth_error types' natIdx).*)
+
+  Definition enD (e : expr types') := natTvarCoerceR (optionDefault (exprD fs' nil nil e natTvar) (natTvarCoerce O)).
+ 
+  Lemma eq_nat_dec_correct : forall n, eq_nat_dec n n = left eq_refl.
+    induction n; provers.
+  Qed.
+  Hint Rewrite eq_nat_dec_correct : provers.
+
+  Lemma nat_seq_dec_correct : forall n, nat_seq_dec n n = Some eq_refl.
+    unfold nat_seq_dec, eq_dec_to_seq_dec in *.
+    provers.
+    autorewrite with provers in *.
+    provers.
+  Qed.
+  Hint Rewrite nat_seq_dec_correct : provers.
+
+  Fixpoint eqGrouper (hyps : list (expr types')) :=
+      match hyps with
+        | nil => nil
+        | hyp :: hyps' => match hyp with
+                            | Func f [x, y] => if eq_nat_dec f eqFunIdx
+                                                 then addEquality (@nat_seq_dec) (eqGrouper hyps') (enD x) (enD y)
+                                                 else eqGrouper hyps'
+                            | _ => eqGrouper hyps'
+                          end
+      end.
+
+  Hint Rewrite inSameGroup_addEquality : provers.
+  Lemma eqGrouper_spec : forall hyps x y, (exists pf, expr_seq_dec x y = Some pf) -> In (Func eqFunIdx [x, y]) hyps -> inSameGroup nat_seq_dec (eqGrouper hyps) (enD x) (enD y) = true.
+    intros.
+    induction hyps; intuition.
+    simpl in *.
+    destruct H, H0.
+    provers.
+    destruct a; intuition.
+    repeat (destruct l; intuition).
+    destruct (eq_nat_dec f eqFunIdx); intuition.
+    apply inSameGroup_addEquality_preserved.
+    assumption.
+  Qed.
+  
+  Lemma eqFunIdx_eq : forall e e', ValidProp fs' (Func eqFunIdx [e, e']) -> exprD fs' nil nil (Func eqFunIdx [e,  e']) tvProp = Some (optionDefault (exprD fs' nil nil e natTvar) (natTvarCoerce 0) = optionDefault (exprD fs' nil nil e' natTvar) (natTvarCoerce 0)).
+    intros.
+    simpl.
+    subst fs'.
+    unfold ValidProp in H.
+    repeat rewrite nth_error_updatePosition in *.
+    simpl in *.
+    repeat rewrite nth_error_updatePosition in *.
+    simpl in *.
+    caseDestruct (exprD (updatePosition fs eqFunIdx eqFunSig) nil nil e natTvar); intuition.
+    caseDestruct (exprD (updatePosition fs eqFunIdx eqFunSig) nil nil e' natTvar); intuition.
+  Qed.
+
+  Lemma nth_error_fs'_eqFunIdx : nth_error fs' eqFunIdx = Some eqFunSig.
+    provers.
+  Qed.
+
+  Lemma Provable_Func_eq : forall e e', Provable fs' nil nil (Func eqFunIdx [e, e']) -> exprD fs' nil nil e natTvar = exprD fs' nil nil e' natTvar.
+    intros.
+    unfold Provable in H.
+    simpl in H.
+    rewrite nth_error_fs'_eqFunIdx in *.
+    simpl in *.
+    destruct (exprD fs' nil nil e natTvar);
+    destruct (exprD fs' nil nil e' natTvar);
+      provers.
+  Qed.
+
+  Hint Resolve groupsEqual_addEquality Provable_Func_eq.
+  Lemma eqGrouper_groupsEqual : forall hyps, AllProvable fs' nil nil hyps -> groupsEqual (eqGrouper hyps).
+    intros.
+    induction hyps; intuition.
+    simpl.
+    destruct a; simpl in *; intuition.
+    repeat (destruct l; simpl in *; intuition).
+    destruct (eq_nat_dec f eqFunIdx).
+    pose (Provable_ValidProp _ _ H0).
+    subst.
+    pose (eqFunIdx_eq v).
+    apply groupsEqual_addEquality.
+    eauto.
+    unfold enD.
+    erewrite Provable_Func_eq; eauto.
+    assumption.
+  Qed.
+
+  Definition transitivityProver (hyps : list (expr types')) (goal : expr types') :=
+    match goal with
+      | Func f [x, y] => if equiv_dec f eqFunIdx
+                           then inSameGroup nat_seq_dec (eqGrouper hyps) (enD x) (enD y)
+                           else false
+      | _ => false
+    end.
+
+  Lemma natTvar_nat : tvarD types' natTvar = nat.
+    provers.
+  Qed.
+
+  Ltac dintuition := repeat (intuition; match goal with
+                                          | [ H : exists _, _ |- _ ] => destruct H
+                                        end).
+  Theorem transitivityProverCorrect : ProverCorrect fs' transitivityProver.
+    unfold ProverCorrect; intros.
+    unfold Provable, transitivityProver in *.
+    caseDestruct goal.
+    repeat caseDestruct l.
+    caseDestruct (equiv_dec f eqFunIdx).
+    unfold equiv in e1.
+    subst.
+    rewrite eqFunIdx_eq; eauto.
+    edestruct inSameGroup_spec; clear H3.
+    specialize (H2 H).
+    apply eqGrouper_groupsEqual in H1.
+    edestruct groupsEqual_spec; clear H4.
+    specialize (H3 H1).
+    unfold ValidProp in *.
+    simpl in *.
+    rewrite nth_error_fs'_eqFunIdx in H0.
+    simpl in *.
+    case_eq (exprD fs' nil nil e natTvar); intros; rewrite H4 in *.
+    case_eq (exprD fs' nil nil e0 natTvar); intros; rewrite H5 in *.
+    dintuition.
+    simpl.
+    unfold enD in *.
+    clear H2.
+    rewrite H4, H5 in x.
+    simpl in *.
+    apply natTvarCoerceR_inj; assumption.
+    dintuition.
+    simpl.
+    specialize (H3 _ H6 _ _ x1 x0).
+    unfold enD in H3.
+    rewrite H4, H5 in *.
+    simpl in *.
+    apply natTvarCoerceR_inj.
+    eauto.
+    tauto.
+    tauto.
+  Qed.
 End BabyOmega.
